src/ext_traversal/ExtTraversalCounting.v
@@ -11,6 +11,8 @@ Require Import ExtTraversal.
 Require Import ExtSimTraversal.
 Require Import ExtSimTraversalProperties.
 
+Require Import IndefiniteDescription.
+
 Set Implicit Arguments.
 Remove Hints plus_n_O.
 
@@ -65,10 +67,26 @@ Section ExtTraversalCounting.
   Notation "'Rel'" := (fun x => is_true (is_rel lab x)).
   Notation "'rmw'" := (rmw G).
 
+
+  (* TODO: get rid while generalizing to infinite case *)
+  (***********)
+  Hypothesis FINDOM: set_finite (acts_set G).  
+  Definition acts_list: list actid :=
+    filterP (acts_set G)
+            (proj1_sig (@constructive_indefinite_description _ _ FINDOM)).
+  Lemma acts_set_findom: acts_set G ≡₁ (fun e => In e acts_list).
+  Proof.
+    unfold acts_list. destruct constructive_indefinite_description. simpl.
+    apply AuxRel.set_equiv_exp_equiv. intros e.
+    rewrite in_filterP_iff. intuition. 
+  Qed.
+  Opaque acts_list.
+  (***********)
+
   Definition trav_steps_left (T : ext_trav_config) :=
-    countP (set_compl (ecovered T)) (acts G) +
-    countP (W ∩₁ set_compl (eissued T)) (acts G) +
-    countP (W ∩₁ set_compl (reserved T)) (acts G).
+    countP (set_compl (ecovered T)) acts_list +
+    countP (W ∩₁ set_compl (eissued T)) acts_list +
+    countP (W ∩₁ set_compl (reserved T)) acts_list.
   
   Lemma trav_steps_left_step_decrease (T T' : ext_trav_config)
         (STEP : ext_trav_step G sc T T') :
@@ -79,8 +97,8 @@ Section ExtTraversalCounting.
     assert (tc_coherent G sc (etc_TC T')) as TCCOH'.
     { apply ETCCOH'. }
     assert (forall e,
-               countP (W ∩₁ set_compl (reserved T)) (acts G) >=
-               countP (W ∩₁ set_compl (reserved T ∪₁ eq e)) (acts G)) as AA.
+               countP (W ∩₁ set_compl (reserved T)) acts_list >=
+               countP (W ∩₁ set_compl (reserved T ∪₁ eq e)) acts_list) as AA.
     { intros e. red. apply countP_mori; auto.
       basic_solver. }
 
@@ -89,33 +107,34 @@ Section ExtTraversalCounting.
     { clear AA.
       unfold trav_steps_left.
       rewrite ISSEQ, RESEQ.
-      assert (countP (set_compl (ecovered T)) (acts G) >
-              countP (set_compl (ecovered T')) (acts G)) as HH.
+      assert (countP (set_compl (ecovered T)) acts_list >
+              countP (set_compl (ecovered T')) acts_list) as HH.
       2: omega.
       eapply countP_strict_mori with (e:=e); auto.
       { rewrite COVEQ. basic_solver. }
       { unfold set_compl. intros HH. apply HH. apply COVEQ. basic_solver. }
-      apply TCCOH'.(coveredE). apply COVEQ. basic_solver. }
+      apply acts_set_findom. 
+      apply (coveredE TCCOH'). apply COVEQ. basic_solver. }
     { unfold trav_steps_left.
       rewrite COVEQ.
       assert (reserved T' e) as RESE.
       { apply RESEQ. basic_solver. }
       assert (W e) as WE by (by apply (reservedW WF ETCCOH')).
-      assert (countP (W ∩₁ set_compl (reserved T )) (acts G) >=
-              countP (W ∩₁ set_compl (reserved T')) (acts G)).
+      assert (countP (W ∩₁ set_compl (reserved T )) acts_list >=
+              countP (W ∩₁ set_compl (reserved T')) acts_list).
       { apply countP_mori; auto. rewrite RESEQ. basic_solver 10. }
-      assert (countP (W ∩₁ set_compl (eissued T )) (acts G) >
-              countP (W ∩₁ set_compl (eissued T')) (acts G)).
+      assert (countP (W ∩₁ set_compl (eissued T )) acts_list >
+              countP (W ∩₁ set_compl (eissued T')) acts_list).
       2: omega.
       apply countP_strict_mori with (e:=e).
       { rewrite ISSEQ. basic_solver. }
       { intros BB. apply BB. apply ISSEQ. basic_solver. }
       { by split. }
-        by apply ETCCOH'.(etc_S_in_E). }
+      apply acts_set_findom. by apply (etc_S_in_E ETCCOH'). }
     unfold trav_steps_left.
     rewrite COVEQ, ISSEQ.
-    assert (countP (W ∩₁ set_compl (reserved T )) (acts G) >
-            countP (W ∩₁ set_compl (reserved T')) (acts G)).
+    assert (countP (W ∩₁ set_compl (reserved T )) acts_list >
+            countP (W ∩₁ set_compl (reserved T')) acts_list).
     2: omega.
     assert (reserved T' e) as RESE.
     { apply RESEQ. basic_solver. }
@@ -124,7 +143,7 @@ Section ExtTraversalCounting.
     { rewrite RESEQ. basic_solver. }
     { intros BB. apply BB. apply RESEQ. basic_solver. }
     { by split. }
-      by apply ETCCOH'.(etc_S_in_E).
+    apply acts_set_findom. by apply (etc_S_in_E ETCCOH').
   Qed.
 
   Lemma trav_steps_left_steps_decrease (T T' : ext_trav_config)
@@ -148,16 +167,16 @@ Section ExtTraversalCounting.
     E ⊆₁ ecovered T.
   Proof using.
     unfold trav_steps_left in *.
-    assert (countP (set_compl (ecovered T)) (acts G) = 0) as HH by omega.
+    assert (countP (set_compl (ecovered T)) acts_list = 0) as HH by omega.
     clear NULL.
     unfold countP in *.
     apply length_zero_iff_nil in HH.
     intros x EX.
     destruct (classic (ecovered T x)) as [|NN]; auto.
     exfalso. 
-    assert (In x (filterP (set_compl (ecovered T)) (acts G))) as UU.
+    assert (In x (filterP (set_compl (ecovered T)) acts_list)) as UU.
     2: { rewrite HH in UU. inv UU. }
-    apply in_filterP_iff. by split.
+    apply in_filterP_iff. split; [by apply acts_set_findom| done].
   Qed.
 
   Lemma trav_steps_left_ncov_nnull (T : ext_trav_config) e
@@ -174,33 +193,33 @@ Section ExtTraversalCounting.
   Proof using.
     assert (tc_coherent G sc (etc_TC T)) as TCCOH by apply ETCCOH.
 
-    assert (countP (set_compl (ecovered T)) (acts G) >=
-            countP (W ∩₁ set_compl (eissued T)) (acts G)) as AA.
+    assert (countP (set_compl (ecovered T)) acts_list >=
+            countP (W ∩₁ set_compl (eissued T)) acts_list) as AA.
     { apply countP_mori; auto.
       intros x [WX NN] COV.
       apply NN. eapply w_covered_issued; eauto. by split. }
 
-    assert (countP (W ∩₁ set_compl (eissued  T)) (acts G) >=
-            countP (W ∩₁ set_compl (reserved T)) (acts G)) as BB.
+    assert (countP (W ∩₁ set_compl (eissued  T)) acts_list >=
+            countP (W ∩₁ set_compl (reserved T)) acts_list) as BB.
     { apply countP_mori; auto.
       intros x [WX NN].
       split; auto. intros CC. apply NN. by apply (etc_I_in_S ETCCOH). }
 
     unfold trav_steps_left in *.
-    assert (countP (set_compl (ecovered T)) (acts G) > 0 \/
-            countP (W ∩₁ set_compl (eissued T)) (acts G) > 0 \/
-            countP (W ∩₁ set_compl (reserved T)) (acts G) > 0) as YY by omega.
-    assert (countP (set_compl (ecovered T)) (acts G) > 0) as HH.
+    assert (countP (set_compl (ecovered T)) acts_list > 0 \/
+            countP (W ∩₁ set_compl (eissued T)) acts_list > 0 \/
+            countP (W ∩₁ set_compl (reserved T)) acts_list > 0) as YY by omega.
+    assert (countP (set_compl (ecovered T)) acts_list > 0) as HH.
     { destruct YY as [|[]]; auto; omega. }
     clear YY.
     unfold countP in HH.
-    assert (exists h l, filterP (set_compl (ecovered T)) (acts G) = h :: l) as YY.
-    { destruct (filterP (set_compl (ecovered T)) (acts G)); eauto.
+    assert (exists h l, filterP (set_compl (ecovered T)) acts_list = h :: l) as YY.
+    { destruct (filterP (set_compl (ecovered T)) acts_list); eauto.
       inv HH. }
     desc. exists h.
-    assert (In h (filterP (set_compl (ecovered T)) (acts G))) as GG.
+    assert (In h (filterP (set_compl (ecovered T)) acts_list)) as GG.
     { rewrite YY. red. by left. }
-    apply in_filterP_iff in GG. simpls.
+    apply in_filterP_iff in GG. generalize acts_set_findom. basic_solver. 
   Qed.
 
   Lemma trav_steps_left_decrease_sim_trans (T T' : ext_trav_config)
@@ -218,7 +237,7 @@ Section ExtTraversalCounting.
         (RELCOV : W ∩₁ Rel ∩₁ eissued T ⊆₁ ecovered T)
         (RMWCOV : forall r w (RMW : rmw r w), ecovered T r <-> ecovered T w) :
     exists T', (ext_sim_trav_step G sc)＊ T T' /\ ((acts_set G) ⊆₁ ecovered T').
-  Proof using WF.
+  Proof using WF FINDOM.
     assert
       (exists T' : ext_trav_config,
           (ext_sim_trav_step G sc)＊ T T' /\ trav_steps_left T' = 0).
@@ -261,7 +280,7 @@ Section ExtTraversalCounting.
   
   Lemma sim_traversal (IMMCON : imm_consistent G sc) :
     exists T, (ext_sim_trav_step G sc)＊ (ext_init_trav G) T /\ ((acts_set G) ⊆₁ ecovered T).
-  Proof using WF.
+  Proof using WF FINDOM.
     apply sim_traversal_helper; auto.
     { by apply ext_init_trav_coherent. }
     { unfold ext_init_trav. simpls. basic_solver. }
@@ -300,7 +319,7 @@ Section ExtTraversalCounting.
         (RELCOV : W ∩₁ Rel ∩₁ eissued T ⊆₁ ecovered T)
         (RMWCOV : forall r w : actid, rmw r w -> ecovered T r <-> ecovered T w) : 
     exists T', (ext_isim_trav_step G sc thread)＊ T T' /\ ((acts_set G) ⊆₁ ecovered T').
-  Proof using WF.
+  Proof using WF FINDOM.
     edestruct sim_traversal_helper as [T']; eauto.
     desc. exists T'. splits; auto.
     clear H0.
@@ -320,4 +339,5 @@ Section ExtTraversalCounting.
     { eapply ext_sim_trav_steps_rel_covered; eauto. }
     eapply ext_sim_trav_steps_rmw_covered; eauto.
   Qed.
+  
 End ExtTraversalCounting.
